examples/NSL_with_properties/DY.NSLP.Invariants.Proofs.fst
@@ -1,0 +1,98 @@
+module DY.NSLP.Invariants.Proofs
+
+open Comparse
+open DY.Core
+open DY.Lib
+
+open DY.Simplified
+open DY.Extend
+
+open DY.NSLP.Data
+open DY.NSLP.Protocol
+open DY.NSLP.Invariants
+
+#set-options "--fuel 0 --ifuel 1 --z3rlimit 25  --z3cliopt 'smt.qi.eager_threshold=100'"
+
+/// In this module, we show that
+/// the protocol steps maintain the protocol invariants.
+///
+/// For every step s we show a lemma of the form:
+/// trace_invariant tr ==> trace_invariant ( trace after step s )
+
+(*** Sending the First Message ***)
+
+
+val send_msg1_invariant:
+  alice:principal -> bob:principal -> alice_public_keys_sid:state_id ->
+  tr:trace ->
+  Lemma
+  ( requires trace_invariant tr
+  )
+  (ensures (
+    let (_ , tr_out) = send_msg1 alice bob alice_public_keys_sid tr in
+    trace_invariant tr_out
+  ))
+let send_msg1_invariant alice bob alice_public_keys_sid tr =
+  let (n_a, tr_rand) = gen_rand_labeled (nonce_label alice bob) tr in
+  let (_, tr_ev) = trigger_event alice (Initiating {alice; bob; n_a}) tr_rand in
+  let msg1 = Msg1 {alice; n_a} in 
+  serialize_wf_lemma message_t (is_knowable_by (nonce_label alice bob) tr_ev) msg1;
+  pke_enc_for_is_publishable tr_ev alice bob alice_public_keys_sid key_tag msg1
+
+(*** Sending the Second Message ***)
+
+
+val decode_msg1_invariant:
+  bob:principal -> bob_private_keys_sid:state_id ->
+  msg:bytes ->
+  tr:trace ->
+  Lemma
+  (requires trace_invariant tr)
+  (ensures (
+    let (_, tr_out) = decode_msg1 bob bob_private_keys_sid msg tr in
+    trace_invariant tr_out
+  ))
+let decode_msg1_invariant bob bob_private_keys_sid msg tr = ()
+
+
+val receive_msg1_and_send_msg2_invariant:
+  bob:principal -> 
+  bob_private_keys_sid:state_id -> bob_public_keys_sid:state_id ->
+  msg_ts:timestamp -> 
+  tr:trace ->
+  Lemma
+  ( requires trace_invariant tr
+  )
+  (ensures (
+    let (_ , tr_out) = receive_msg1_and_send_msg2 bob bob_private_keys_sid bob_public_keys_sid msg_ts tr in
+    trace_invariant tr_out
+  ))
+let receive_msg1_and_send_msg2_invariant bob bob_private_keys_sid bob_public_keys_sid msg_ts tr =
+  match recv_msg msg_ts tr with
+  | (None, _ ) -> ()
+  | (Some msg, _) -> (
+      match decode_msg1 bob bob_private_keys_sid msg tr with
+      | (None, _) -> ()
+      | (Some {alice; n_a}, tr_decode) -> (
+          assert(trace_invariant tr_decode);
+          let (n_b, tr_rand) = gen_rand_labeled (nonce_label alice bob) tr in
+          assert(trace_invariant tr_rand);
+          let (_, tr_ev) = trigger_event bob (Responding1 {alice; bob; n_a; n_b}) tr_rand in
+          assert(trace_invariant tr_ev);
+          let msg2 = Msg2 {bob; n_a; n_b} in
+          match pke_enc_for bob alice bob_public_keys_sid key_tag msg2 tr_ev with
+          | (None, _) -> ()
+          | (Some msg2_encrypted, tr_msg2) ->(
+              assert(trace_invariant tr_msg2);
+              let (msg2_ts, tr_msg2) = send_msg msg2_encrypted tr_msg2 in
+              assume(trace_invariant tr_msg2);
+              let state = SentMsg2 {alice; n_a; n_b} in
+              let (sess_id, tr_sess) = start_new_session bob state tr_msg2 in
+              assume(trace_invariant tr_sess)
+          )
+      )
+  )
+
+(*** Sending the Third Message ***)
+
+(*** Receiving the Final Message ***)
